examples/tactics/Syntax.fst
@@ -1,0 +1,28 @@
+module Syntax
+
+open FStar.Tactics
+
+let blah : term -> tactic term = fix1 (fun ff t ->
+    tv <-- inspect t;
+    tv <-- (match tv with
+           | Tv_Var b -> return (Tv_Var b)
+           | Tv_FVar f -> return (Tv_FVar f)
+           | Tv_App l r -> l <-- ff l;
+                           r <-- ff r;
+                           return (Tv_App l r)
+           | Tv_Abs b t -> t <-- ff t;
+                           return (Tv_Abs b t)
+           | Tv_Arrow b t -> t <-- ff t;
+                             return (Tv_Arrow b t)
+           | Tv_Refine b t -> t <-- ff t;
+                              return (Tv_Refine b t)
+           | Tv_Type u -> return (Tv_Type ())
+           | Tv_Const c -> return (Tv_Const c));
+    pack tv)
+
+let _ = assert_by_tactic (t <-- quote (1+1);
+                          s <-- term_to_string t; print ("t = " ^ s);;
+                          t <-- blah t;
+                          s <-- term_to_string t; print ("t = " ^ s);;
+                          return ()
+                          ) (True)
